examples/crypto/mac.fst
@@ -18,52 +18,6 @@
    hashes, namely HMAC-SHA1, and their idealization under the INT-CMA
    computational assumption *)
 
-
-
-
-
-
-(* module List *)
-(* assume val find: a:Type *)
-(*         -> f:(a -> Tot bool) *)
-(*         -> list a *)
-(*         -> Tot (option (x:a{f x})) *)
-
-
-
-module SHA1
-open Array
-
-type bytes = seq byte (* concrete byte arrays *)
-type text  = bytes    (* a type abbreviation, for clarity *)
-
-type nbytes (n:nat) =
-  b:bytes{length b == n} (* fixed-length bytes *)
-
-(* we rely on some external crypto library implementing HMAC-SHA1 *)
-
-let keysize = 16
-let macsize = 20
-
-type key = nbytes keysize
-type tag = nbytes macsize
-
-assume val sample: n:nat -> nbytes n
-assume val sha1: key -> text -> Tot tag
-
-
-(* to verify, we simply recompute & compare *)
-
-val sha1verify: key -> text -> tag -> Tot bool
-let sha1verify k txt tag = (sha1 k txt = tag)
-
-
-
-
-
-
-
-
 module MAC
 open Array
 open SHA1
