examples/crypto/rpc.fst
@@ -3,13 +3,15 @@
 module RPC
 open Array
 open SHA1
-open Format
+open Formatting
 open MAC
 
 (* some basic, untrusted network controlled by the adversary *)
 
-assume val send: message -> unit
-assume val recv: (message -> unit) -> unit
+val send: message -> unit
+let send m = magic()
+val recv: (message -> unit) -> unit
+let recv m = magic()
 
 (* two events, recording genuine requests and responses *)
 
@@ -19,20 +21,20 @@ logic type Response : string -> string -> Type
 (* the meaning of MACs, as used in RPC *)
 
 opaque logic type reqresp (msg:message) =
-    (exists s.   msg = Format.request s    /\ Request s)
- \/ (exists s t. msg = Format.response s t /\ Response s t)
+    (exists s.   msg = Formatting.request s    /\ Request s)
+ \/ (exists s t. msg = Formatting.response s t /\ Response s t)
 
 let k = keygen reqresp 
 
 let client (s:string16) =
   assume (Request s);
-  send (append (utf8 s) (mac k (Format.request s))); 
+  send (append (utf8 s) (mac k (Formatting.request s))); 
   recv (fun msg ->
     if length msg < macsize then failwith "Too short"
     else
       let (v, m') = split msg (length msg - macsize) in
       let t = iutf8 v in
-      if verify k (Format.response s t) m'
+      if verify k (Formatting.response s t) m'
       then assert (Response s t))
 
 let server () =
@@ -43,12 +45,12 @@ let server () =
       if length v > 65535 then failwith "Too long" 
       else
         let s = iutf8 v in
-        if verify k (Format.request s) m 
+        if verify k (Formatting.request s) m 
         then  
           ( assert (Request s);
             let t = "22" in
             assume (Response s t);
-            send (append (utf8 t) (mac k (Format.response s t)))))
+            send (append (utf8 t) (mac k (Formatting.response s t)))))
   
 (* 
 let test () = 
