examples/crypto/sha1.fst
@@ -1,0 +1,26 @@
+module SHA1
+open Array
+
+type bytes = seq byte (* concrete byte arrays *)
+type text  = bytes    (* a type abbreviation, for clarity *)
+
+type nbytes (n:nat) =
+  b:bytes{length b == n} (* fixed-length bytes *)
+
+(* we rely on some external crypto library implementing HMAC-SHA1 *)
+
+let keysize = 16
+let macsize = 20
+
+type key = nbytes keysize
+type tag = nbytes macsize
+
+val sample: n:nat -> nbytes n
+let sample n = magic()
+val sha1: key -> text -> Tot tag
+let sha1 k t = magic()
+
+(* to verify, we simply recompute & compare *)
+
+val sha1verify: key -> text -> tag -> Tot bool
+let sha1verify k txt tag = (sha1 k txt = tag)
